veric/semax_loop.v
@@ -350,16 +350,16 @@ destruct ek; try congruence; auto.
 Qed.
 
 Lemma semax_for : 
-forall Delta Q Q' test incr body R
-     (TC: forall rho, Q rho |-- tc_expr Delta test rho)
-     (BT: bool_type (Clight.typeof test) = true) (*Is used, probably needed*)
-     (POST: forall rho,  !! expr_false (test) rho && Q rho |-- R EK_normal nil rho),
+forall Delta Q Q' test incr body R,
+     bool_type (Clight.typeof test) = true ->
+     (forall rho, Q rho |-- tc_expr Delta test rho) ->
+     (forall rho,  !! expr_false (test) rho && Q rho |-- R EK_normal nil rho) ->
      semax Hspec Delta
                 (fun rho => !! expr_true test rho && Q rho) body (for1_ret_assert Q' R) ->
      semax Hspec Delta Q' incr (for2_ret_assert Q R) ->
      semax Hspec Delta Q (Sfor' test incr body) R.
 Proof.
-intros.
+intros ? ? ? ? ? ? ? BT TC POST H H0.
 rewrite semax_unfold.
 intros until 2.
 rename H1 into H2.
@@ -542,19 +542,19 @@ Qed.
 
 
 Lemma semax_while : 
-forall Delta Q test body R
-     (TC: forall rho, Q rho |-- tc_expr Delta test rho)
-     (BT: bool_type (Clight.typeof test) = true) 
-     (POST: forall rho,  !! (expr_false test rho) && Q rho |-- R EK_normal nil rho),
+forall Delta Q test body R,
+     bool_type (Clight.typeof test) = true ->
+    (forall rho, Q rho |-- tc_expr Delta test rho) ->
+     (forall rho,  !! (expr_false test rho) && Q rho |-- R EK_normal nil rho) ->
      semax Hspec Delta 
                 (fun rho => !! expr_true test rho && Q rho) body (for1_ret_assert Q R) ->
      semax Hspec Delta Q (Swhile test body) R.
 Proof.
-intros.
+intros ? ? ? ? ? BT TC POST H.
 assert (semax Hspec Delta Q Sskip (for2_ret_assert Q R)).
 eapply semax_post; try apply semax_Sskip.
 destruct ek; unfold normal_ret_assert, for2_ret_assert; intros; normalize; inv H0; try discriminate.
-pose proof (semax_for Delta Q Q test Sskip body R TC BT POST H H0).
+pose proof (semax_for Delta Q Q test Sskip body R BT TC POST H H0).
 clear H H0.
 rewrite semax_unfold in H1|-*.
 rename H1 into H0; pose (H:=True).
